More work in src/ByteStringHeap.v

src/ByteStringHeap.v
@@ -19,26 +19,38 @@ Require Import
 
 Generalizable All Variables.
 
-Open Scope N_scope.
+Theorem Nlt_plus_1 : forall n : N, 0 < n + 1.
+Proof. nomega. Qed.
 
-(*
-Lemma within_index : forall addr len i,
-  (i <? len) -> within addr len (addr + i).
+Corollary refine_computes_to_ret :
+  forall A f (v : A), f ↝ v <-> refine f (ret v).
 Proof.
-  intros.
-  split.
-    apply N.le_add_r.
-  apply N.add_lt_mono_l.
-  apply N.ltb_lt.
-  assumption.
+  split; intros.
+    apply refine_In.
+    exact H.
+  apply H.
+  constructor.
 Qed.
-*)
+
+Lemma refineEquiv_If_Then_Else_Bind :
+  forall (A B : Type) (i : bool) (t e : Comp A) (b : A -> Comp B),
+    refineEquiv (a <- If i Then t Else e; b a)
+                (If i Then a <- t; b a Else (a <- e; b a)).
+Proof. split; intros; destruct i; reflexivity. Qed.
+
+Theorem refine_If_Then_Else_bool :
+  forall (b : bool) A cpst cpse (res : Comp A),
+    (if b then refine cpst res else refine cpse res)
+      <-> refine (If b Then cpst Else cpse) res.
+Proof. split; intros; destruct b; auto. Qed.
 
 Module ByteStringHeap (Mem : Memory).
 
 Module Import BS := ByteString Mem.
 Module Import Adt := HeapADT Mem.
 Import Heap.
+
+Open Scope N_scope.
 
 Definition HSpec := projT1 HeapSpecADT.
 
@@ -68,113 +80,172 @@ Record PS := makePS {
   psLength : N
 }.
 
-Record Correct (ps : PS) : Prop := {
-  _ : psOffset ps + psLength ps <= psBufLen ps;
-  _ : 0 < psBufLen ps -> exists data,
-        Lookup (psBuffer ps) {| memSize := psBufLen ps
-                              ; memData := data |} (` (psHeap ps))
-}.
+Definition poke_at_offset (r : PS) (d : Mem.Word8) : Comp PS :=
+  res <- poke' (psHeap r) (psBuffer r + psOffset r) d;
+  ret {| psHeap   := fst res
+       ; psBuffer := psBuffer r
+       ; psBufLen := psBufLen r
+       ; psOffset := psOffset r
+       ; psLength := psLength r |}.
 
-Theorem Nlt_plus_1 : forall n : N, 0 < n + 1.
-Proof. nomega. Qed.
+Definition simply_widen_region (r : PS) : PS :=
+  {| psHeap   := psHeap r
+   ; psBuffer := psBuffer r
+   ; psBufLen := psBufLen r
+   ; psOffset := psOffset r - 1
+   ; psLength := psLength r + 1 |}.
+
+Definition make_room_by_shifting_up (r : PS) : Comp PS :=
+  res <- memcpy' (psHeap r) (psBuffer r) (psBuffer r + 1)
+                 (psLength r);
+  ret {| psHeap   := fst res
+       ; psBuffer := psBuffer r
+       ; psBufLen := psBufLen r
+       ; psOffset := 0
+       ; psLength := psLength r + 1 |}.
+
+Definition make_room_by_growing_buffer (r : PS) : Comp PS :=
+  (* jww (2016-06-28): We could make a trade-off here by allocating
+     extra bytes at the beginning in anticipation of future calls to
+     [buffer_cons]. *)
+  res <- realloc' (psHeap r) (psBuffer r)
+                  (exist _ (psLength r + 1) (Nlt_plus_1 _));
+  ret {| psHeap   := fst res
+       ; psBuffer := snd res
+       ; psBufLen := psLength r + 1
+       ; psOffset := 0
+       ; psLength := psLength r + 1 |}.
 
 Definition buffer_cons (r : PS) (d : Mem.Word8) : Comp PS :=
   ps <- If 0 <? psOffset r
-        Then ret {| psHeap   := psHeap r
-                  ; psBuffer := psBuffer r
-                  ; psBufLen := psBufLen r
-                  ; psOffset := psOffset r - 1
-                  ; psLength := psLength r + 1 |}
+        Then ret (simply_widen_region r)
         Else If psLength r <? psBufLen r
-        Then (
-          res <- memcpy' (psHeap r) (psBuffer r) (psBuffer r + 1)
-                         (psLength r);
-          ret {| psHeap   := fst res
-               ; psBuffer := psBuffer r
-               ; psBufLen := psBufLen r
-               ; psOffset := 0
-               ; psLength := psLength r + 1 |})
-        Else (
-          (* jww (2016-06-28): We could make a trade-off here by allocating
-             extra bytes at the beginning in anticipation of future calls to
-             [buffer_cons]. *)
-          res <- realloc' (psHeap r) (psBuffer r)
-                          (exist _ (psLength r + 1) (Nlt_plus_1 _));
-          ret {| psHeap   := fst res
-               ; psBuffer := snd res
-               ; psBufLen := psLength r + 1
-               ; psOffset := 0
-               ; psLength := psLength r + 1 |});
-  res <- poke' (psHeap ps) (psBuffer ps + psOffset ps) d;
-  ret {| psHeap   := fst res
-       ; psBuffer := psBuffer ps
-       ; psBufLen := psBufLen ps
-       ; psOffset := psOffset ps
-       ; psLength := psLength ps |}.
+             Then make_room_by_shifting_up r
+             Else make_room_by_growing_buffer r;
+  poke_at_offset ps d.
 
-Lemma refine_ret_eq_r : forall A (a b : A), refine (ret a) (ret b) -> a = b.
+Ltac tease_apart_binds :=
+  repeat match goal with
+  | [ H : _ ↝ _ |- _ ] =>
+    apply Bind_inv in H;
+    destruct H as [? [? H]];
+    apply Return_inv in H;
+    rewrite <- H; simpl
+  | [ H : _ ↝ _ |- _ ] =>
+    apply Bind_dep_inv in H;
+    destruct H as [? [? H]];
+    apply Return_inv in H;
+    rewrite <- H; simpl
+  end.
+
+Lemma buffer_cons_ind : forall (R1 R2 R3 R : relation PS) ps d ps',
+     (0 < psOffset ps -> R1 ps (simply_widen_region ps))
+  -> (forall v,
+        psOffset ps = 0
+          -> psLength ps < psBufLen ps
+          -> make_room_by_shifting_up ps ↝ v
+          -> R2 ps v)
+  -> (forall v,
+        psOffset ps = 0
+          -> psLength ps >= psBufLen ps
+          -> make_room_by_growing_buffer ps ↝ v
+          -> R3 ps v)
+  -> (forall v v' v'',
+        (R1 v v' \/ R2 v v' \/ R3 v v')
+          -> 0 < psLength v'
+          -> poke_at_offset v' d ↝ v''
+          -> R v v'')
+  -> buffer_cons ps d ↝ ps'
+  -> R ps ps'.
 Proof.
-  intros.
-  specialize (H b (ReturnComputes b)).
-  apply Return_inv; assumption.
+  intros R1 R2 R3 R ? ? H1 H2 H3 H4 H5 H.
+  unfold buffer_cons in H.
+  apply refine_computes_to_ret in H.
+  rewrite refineEquiv_If_Then_Else_Bind in H.
+  apply refine_If_Then_Else_bool in H.
+  destruct (0 <? psOffset ps) eqn:Heqe.
+    apply refine_computes_to_ret in H.
+    {
+      apply Bind_inv in H.
+      destruct H, H.
+      apply Return_inv in H.
+      apply H5 with (v':=x); subst.
+      - left; apply H2; nomega.
+      - nomega.
+      - nomega.
+    }
+  rewrite refineEquiv_If_Then_Else_Bind in H.
+  apply refine_If_Then_Else_bool in H.
+  destruct (psLength ps <? psBufLen ps) eqn:Heqe2;
+  apply refine_computes_to_ret in H.
+  {
+    apply Bind_inv in H.
+    destruct H, H.
+    apply H5 with (v':=x).
+    - right; left.
+      apply H3; nomega.
+    - tease_apart_binds; nomega.
+    - assumption.
+  }
+  {
+    apply Bind_inv in H.
+    destruct H, H.
+    apply H5 with (v':=x).
+    - right; right.
+      apply H4, H; nomega.
+    - tease_apart_binds; nomega.
+    - assumption.
+  }
 Qed.
 
-Theorem If_Then_Else_correct :
-  forall b cpst cpse ps',
-    (forall pst, b = true -> refine cpst (ret pst) -> Correct pst) ->
-    (forall pse, b = false -> refine cpse (ret pse) -> Correct pse) ->
-    refine (If b
-            Then cpst
-            Else cpse) (ret ps') -> Correct ps'.
-Proof.
-  intros.
-  specialize (H1 ps' (ReturnComputes ps')).
-  destruct b; simpl in *;
-  [ apply H | apply H0 ]; auto;
-  intros ??;
-  apply Return_inv in H2; subst;
-  assumption.
-Qed.
+Tactic Notation "unfold_buffer_cons" constr(R1) constr(R2) constr(R3) :=
+  repeat match goal with
+  | [ H : buffer_cons ?PS ?D ↝ ?PS' |- _ ] =>
+    apply (buffer_cons_ind R1 R2 R3)
+      with (ps:=PS) (d:=D) (ps':=PS'); intuition
+  | [ H : _ ↝ _ |- _ ] => tease_apart_binds
+  end.
 
-Theorem poke'_correct `(_ : Correct ps) : forall offset length d ps',
-  0 < length ->
-  offset + length <= psBufLen ps ->
-  refine (res <- poke' (psHeap ps) (psBuffer ps + offset) d;
-          ret {| psHeap   := fst res
-               ; psBuffer := psBuffer ps
-               ; psBufLen := psBufLen ps
-               ; psOffset := offset
-               ; psLength := length |}) (ret ps') -> Correct ps'.
+Theorem buffer_cons_length_increase ps : forall ps' x,
+  buffer_cons ps x ↝ ps' -> psLength ps' = psLength ps + 1.
 Proof.
-  intros ??????.
-  unfold poke', poke.
-  rewrite refine_bind_dep_bind_ret; simpl.
-  rewrite refine_bind_dep_ret; simpl.
-  intro H1.
-  apply refine_ret_eq_r in H1.
-  subst; simpl.
-  destruct Correct0.
-  constructor; simpl; [nomega|].
-  intuition; destruct_ex.
-  exists (Update offset d x).
-  teardown.
-  exists {| memSize := psBufLen ps; memData := x |}; simpl.
-  decisions; intuition; f_equal.
-    f_equal; nomega.
-  nomega.
+  intros;
+  set (P := fun x x' => psLength x = psLength x' - 1).
+  unfold_buffer_cons P P P; unfold P in *; nomega.
 Qed.
 
 Definition buffer_uncons (r : PS) : Comp (PS * option Mem.Word8) :=
-  If 0 <? psLength r
-  Then (
+  If psLength r =? 0
+  Then ret (r, None)
+  Else (
     w <- peek' (psHeap r) (psBuffer r + psOffset r);
     ret ({| psHeap   := psHeap r
           ; psBuffer := psBuffer r
           ; psBufLen := psBufLen r
           ; psOffset := psOffset r + 1
-          ; psLength := psLength r - 1 |}, Some (snd w))
-  )
-  Else ret (r, None).
+          ; psLength := psLength r - 1 |}, Some (snd w))).
+
+Definition list_to_set {A} (xs : list A) : Ensemble A :=
+  fold_right (fun x rest => Add _ rest x) (Empty_set _) xs.
+
+Definition number_list {A} (base : N) (xs : list A) : list (N * A) :=
+  snd (fold_right (fun x (p : N * list (N * A)) =>
+                     let (n, rest) := p in
+                     (N.succ n, (n, x) :: rest)) (base, []) xs).
+
+Definition list_map_rel {A} (base : N) (xs : list A) : EMap N A -> Prop :=
+  Same (list_to_set (number_list base xs)).
+
+Definition ByteString_list_AbsR (or : Rep ByteStringSpec) `(nr : PS) :=
+  length or = N.to_nat (psLength nr) /\
+  IF psLength nr = 0
+  then psBufLen nr = 0 /\ psOffset nr = 0
+  else exists data,
+    Lookup (psBuffer nr) {| memSize := psBufLen nr; memData := data |}
+           (` (psHeap nr))
+      /\ list_map_rel (psOffset nr) or
+                      (Filter (fun k _ => within (psOffset nr)
+                                                 (psLength nr) k) data).
 
 Global Program Instance refineEquiv_bind_dep : forall A (ca : Comp A) B,
   Proper (forall_relation
@@ -193,72 +264,6 @@ Obligation 1.
   eapply H in c; eauto.
 Qed.
 
-Lemma refineEquiv_If_Then_Else_Bind :
-  forall (A B : Type) (i : bool) (t e : Comp A) (b : A -> Comp B),
-    refineEquiv (a <- If i Then t Else e; b a)
-                (If i Then a <- t; b a Else (a <- e; b a)).
-Proof. split; intros; destruct i; reflexivity. Qed.
-
-Theorem buffer_cons_correct `(_ : Correct ps) : forall ps' x,
-  refine (buffer_cons ps x) (ret ps') -> Correct ps'.
-Proof.
-  unfold buffer_cons; intros.
-  revert H.
-  rewrite refineEquiv_If_Then_Else_Bind.
-  apply If_Then_Else_correct; intros ??.
-    autorewrite with monad laws; simpl.
-    apply poke'_correct; trivial.
-      nomega.
-    destruct Correct0.
-    nomega.
-  rewrite refineEquiv_If_Then_Else_Bind.
-  apply If_Then_Else_correct; intros ??.
-    autorewrite with monad laws; simpl.
-    admit.
-  autorewrite with monad laws; simpl.
-  admit.
-Admitted.
-
-Theorem buffer_cons_length_increase ps : forall ps' x,
-  buffer_cons ps x ↝ ps' -> psLength ps' = psLength ps + 1.
-Proof.
-  unfold buffer_cons, peek, poke, memcpy in *.
-  destruct (0 <? psOffset ps) eqn:Heqe;
-  destruct (psLength ps <? psBufLen ps);
-  simpl; intros; clear -H; simpl in H;
-  simplify_ensembles; subst; simpl;
-  reflexivity.
-Qed.
-
-(*
-Theorem buffer_cons_data_retained `(_ : Correct ps) : forall ps' x,
-  buffer_cons ps x ↝ ps' ->
-    (x <- peek (` (psHeap ps')) (psOffset ps'); ret (snd x)) ↝ x /\
-    forall i,
-      refineEquiv
-        (x <- peek (` (psHeap ps')) (psOffset ps' + (i + 1)); ret (snd x))
-        (x <- peek (` (psHeap ps)) (psOffset ps + i); ret (snd x)).
-Proof.
-  unfold buffer_cons, peek, poke, memcpy in *.
-  destruct (0 <? psOffset ps) eqn:Heqe;
-  destruct (psLength ps <? psBufLen ps);
-  simpl; intros; clear -H Heqe; simpl in H;
-  simplify_ensembles; subst; simpl;
-  autorewrite with monad laws;
-  simplify_ensembles; subst; simpl;
-  intros; reduction.
-*)
-
-Definition ByteString_list_AbsR (or : Rep ByteStringSpec) `(nr : PS) :=
-     (* then the list and active region must be the same size *)
-     length or = N.to_nat (psLength nr)
-     (* and for every index within the list... *)
-  /\ forall i, (i <? length or)%nat
-     (* each byte in the list matches its corresponding byte in the buffer. *)
-       -> forall x, x = nth i or x
-          <-> (x <- peek (` (psHeap nr)) (psOffset nr + N.of_nat i);
-               ret (snd x)) ↝ x.
-
 Theorem buffer_cons_sound
         (r_o : list Mem.Word8) (r_n : PS)
         (AbsR : ByteString_list_AbsR r_o r_n) :
@@ -266,13 +271,114 @@ Theorem buffer_cons_sound
     ByteString_list_AbsR (x :: r_o) r_n'.
 Proof.
   intros.
-  split; intros.
-    apply buffer_cons_length_increase in H.
-    destruct AbsR; nomega.
-  split; intros.
-    rewrite H1; clear H1.
-    admit.
-  admit.
+(*
+  right.
+  split; [nomega|].
+  destruct AbsR.
+    destruct H0, H1, H2.
+    exists (Update 0 x Empty).
+    split.
+      revert H.
+      unfold buffer_cons, make_room_by_growing_buffer, poke_at_offset.
+      rewrite H1, H2, H3; simpl; clear H1 H2 H3.
+      unfold realloc'.
+      rewrite refine_bind_dep_bind_ret; simpl.
+      rewrite refine_bind_dep_bind_ret; simpl.
+      unfold poke'; simpl.
+      setoid_rewrite refine_bind_dep_bind_ret; simpl.
+      intros.
+      apply Bind_dep_inv in H.
+      destruct H, H.
+      apply Bind_dep_inv in c.
+      destruct c, H.
+      apply Return_inv in c.
+      destruct r_n';
+      tsubst; simpl in *.
+      inv c; simpl.
+      apply Return_inv in x3; subst; simpl.
+      teardown.
+      exists {| memSize := 1; memData := Empty |}; simpl.
+      rewrite N.add_0_r.
+      assert (within (snd x0) 1 (snd x0)) by nomega.
+      unfold IfDec_Then_Else; simpl.
+      apply within_reflect in H; rewrite H.
+      intuition.
+      f_equal; f_equal.
+      nomega.
+      unfold poke in x3.
+  destruct H0, H1.
+  exists (Update (psOffset r_n') x x0).
+*)
+(*
+  revert AbsR.
+  apply
+    (buffer_cons_ind
+       (fun r_n r_n' =>
+          r_n' = {| psHeap   := psHeap   r_n
+                  ; psBuffer := psBuffer r_n
+                  ; psBufLen := psBufLen r_n
+                  ; psOffset := psOffset r_n - 1
+                  ; psLength := psLength r_n + 1 |})
+       (fun r_n r_n' =>
+          exists h,
+          memcpy' (psHeap r_n) (psBuffer r_n) (psBuffer r_n + 1)
+                  (psLength r_n) ↝ h /\
+          r_n' = {| psHeap   := fst h
+                  ; psBuffer := psBuffer r_n
+                  ; psBufLen := psBufLen r_n
+                  ; psOffset := 0
+                  ; psLength := psLength r_n + 1 |})
+       (fun r_n r_n' =>
+          exists h,
+          realloc' (psHeap r_n) (psBuffer r_n)
+                   (exist (N.lt 0) (psLength r_n + 1)
+                          (Nlt_plus_1 (psLength r_n))) ↝ h /\
+          r_n' = {| psHeap   := fst h
+                  ; psBuffer := snd h
+                  ; psBufLen := psLength r_n + 1
+                  ; psOffset := 0
+                  ; psLength := psLength r_n + 1 |}))
+   with (ps:=r_n) (ps':=r_n') (d:=x);
+  intros; trivial;
+  destruct r_n; simpl in *;
+  f_equal; try nomega;
+  tease_apart_binds;
+  simpl in *; subst.
+  - remember (exist _ _ _) as E.
+    exists (E, snd x1).
+    split; trivial.
+    rewrite HeqE.
+    exists x1.
+    exists x2.
+    constructor.
+  - remember (exist _ (fst x1) _) as E.
+    exists (E, snd x1).
+    split; trivial.
+    rewrite HeqE.
+    exists x1.
+    exists x2.
+    constructor.
+  - destruct H0.
+      subst; simpl in *.
+      unfold ByteString_list_AbsR in *; simpl in *.
+      left.
+      destruct AbsR.
+        admit.
+      destruct H0, H2.
+      split.
+        nomega.
+      rewrite H2, H3 in *; simpl.
+      exists Empty.
+    destruct H0.
+      destruct H0, H0.
+      subst; simpl in *.
+      unfold ByteString_list_AbsR in *; simpl in *.
+      admit.
+    destruct H0, H0.
+      subst; simpl in *.
+      unfold ByteString_list_AbsR in *; simpl in *.
+      admit.
+*)
 Admitted.
 
 Theorem buffer_uncons_sound
@@ -285,16 +391,62 @@ Theorem buffer_uncons_sound
                           end) r_n'.
 Proof.
   intros.
-  split; intros.
-    admit.
-  split; intros.
-    admit.
-  admit.
 Admitted.
 
-Lemma ByteStringImpl (heap : Rep HSpec) : FullySharpened ByteStringSpec.
+Lemma refine_ret_eq_r : forall A (a b : A), refine (ret a) (ret b) -> a = b.
 Proof.
-  start sharpening ADT.
+  intros.
+  specialize (H b (ReturnComputes b)).
+  apply Return_inv; assumption.
+Qed.
+
+Theorem buffer_uncons_impl : forall r_o r_n a,
+  ByteString_list_AbsR r_o r_n
+    -> buffer_uncons r_n ↝ a
+    -> match snd a with
+       | Some w => exists r_o', r_o = w :: r_o'
+       | None => r_o = []
+       end.
+Proof.
+  unfold buffer_uncons; intros.
+  apply refine_computes_to_ret in H0.
+  apply refine_If_Then_Else_bool in H0.
+  destruct (psLength r_n =? 0) eqn:Heqe.
+    apply refine_ret_eq_r in H0.
+    destruct a; tsubst; simpl in *.
+    destruct H, H0, H0.
+      destruct r_o; simpl in *; auto.
+      rewrite H0 in H; simpl in H.
+      discriminate.
+    destruct r_o; simpl in *; auto.
+    nomega.
+  revert H0.
+  unfold peek'.
+  rewrite refine_bind_dep_bind_ret; simpl.
+  rewrite refine_bind_dep_ignore.
+  unfold peek.
+  autorewrite with monad laws; simpl.
+  intros.
+  apply refine_computes_to_ret in H0.
+  apply Bind_inv in H0.
+  destruct H0, H0.
+  apply Return_inv in H1.
+  destruct a; tsubst; simpl in *.
+  apply Pick_inv in H0.
+  destruct H.
+  destruct H1.
+    nomega.
+  destruct H1, H2, H2.
+  specialize (H0 _ _ H2); simpl in *.
+Admitted.
+
+Section Refined.
+
+Variable heap : Rep HSpec.
+
+Lemma ByteStringHeap  : { adt : _ & refineADT ByteStringSpec adt }.
+Proof.
+  eexists.
   hone representation using ByteString_list_AbsR.
   {
     simplify with monad laws.
@@ -305,9 +457,7 @@ Proof.
        ; psOffset := 0
        ; psLength := 0 |}.
       finish honing.
-    split; intros.
-      reflexivity.
-    split; intros; discriminate.
+    right; simpl; intuition.
   }
   {
     simplify with monad laws.
@@ -319,7 +469,8 @@ Proof.
         simplify with monad laws.
         finish honing.
       eapply buffer_cons_sound; eauto.
-    unfold buffer_cons.
+    unfold buffer_cons, simply_widen_region,
+           make_room_by_shifting_up, make_room_by_growing_buffer.
     simplify with monad laws; simpl.
     finish honing.
   }
@@ -329,22 +480,42 @@ Proof.
       eapply (refine_skip2 (dummy:=buffer_uncons r_n)).
     etransitivity.
       apply refine_under_bind; intros; simpl.
+      pose proof H1.
+      eapply buffer_uncons_impl in H1; eauto.
       refine pick val (fst a).
         simplify with monad laws.
         finish honing.
       pose proof (buffer_uncons_sound H0 (snd a) (fst a)).
-      rewrite <- surjective_pairing in H2.
-      specialize (H2 H1).
-      destruct a; simpl in *.
-      simpl.
-      admit.
+      rewrite <- surjective_pairing in H3.
+      specialize (H3 H2).
+      destruct (snd a); simpl in *.
+        destruct H1; subst; assumption.
+      subst; assumption.
+    simpl.
+    etransitivity.
+      eapply refine_under_bind; intros; simpl.
+      replace (snd match r_o with
+                   | [] => (r_o, None)
+                   | x :: xs => (xs, Some x)
+                   end)
+          with (snd a).
+        rewrite <- surjective_pairing.
+        finish honing.
+      eapply buffer_uncons_impl in H1; eauto.
+      destruct (snd a).
+        destruct H1; subst.
+        reflexivity.
+      subst; reflexivity.
+    simplify with monad laws; simpl.
     unfold buffer_uncons.
-    admit.
+    finish honing.
   }
-  finish_SharpeningADT_WithoutDelegation.
-Admitted.
+  apply reflexivityT.
+Defined.
 
-Fail Definition ByteStringImpl' := Eval simpl in projT1 ByteStringImpl.
-(* Print ByteStringImpl'. *)
+Definition ByteStringHeap' := Eval simpl in projT1 ByteStringHeap.
+Print ByteStringHeap'.
+
+End Refined.
 
 End ByteStringHeap.
